

Assignment 5: Solutions

CS 750/850 Machine Learning

Problem 1 [33%]

It is mentioned in Chapter 7 of ISL that a cubic regression spline with one knot at ξ can be obtained using a basis of the form $x, x^2, x^3, [x - \xi]_+^3$, where $[x - \xi]_+^3 = (x - \xi)^3$ if $x > \xi$ and equals 0 otherwise. We will now show that a function of the form

$$f(x) = \beta_0 + \beta_1 x + \beta_2 x^2 + \beta_3 x^3 + \beta_4 [x - \xi]_+^3$$

is indeed a cubic regression spline, regardless of the values of $\beta_0, \beta_1, \beta_2, \beta_3, \beta_4$.

1. Find a cubic polynomial

$$f_1(x) = a_1 + b_1 x + c_1 x^2 + d_1 x^3$$

such that $f(x) = f_1(x)$ for all $x \leq \xi$. Express a_1, b_1, c_1, d_1 in terms of $\beta_0, \beta_1, \beta_2, \beta_3, \beta_4$.

2. Find a cubic polynomial

$$f_2(x) = a_2 + b_2 x + c_2 x^2 + d_2 x^3$$

such that $f(x) = f_2(x)$ for all $x > \xi$. Express a_2, b_2, c_2, d_2 in terms of $\beta_0, \beta_1, \beta_2, \beta_3, \beta_4$. We have now established that $f(x)$ is a piece-wise polynomial.

3. Show that $f_1(\xi) = f_2(\xi)$. That is, $f(x)$ is continuous at ξ .

Solution

1. The values are:

$$a_1 = \beta_0, \quad b_1 = \beta_1, \quad c_1 = \beta_2, \quad d_1 = \beta_3$$

2. Recall that:

$$(x - \xi)^3 = x^3 - \xi^3 + 3x\xi^2 - 3x^2\xi$$

Then, the values are:

$$a_2 = (\beta_0 - \beta_4 \xi^3),$$

$$b_2 = (\beta_1 + 3\beta_4 \xi^2),$$

$$c_2 = (\beta_2 - 3\beta_4 \xi),$$

$$d_2 = \beta_3 + \beta_4$$

3. Follows by algebraic manipulation, or simply from the fact that $[x - \xi]^3 = 0$ when $x = \xi$.

It is mentioned in Chapter 7 of ISL that a cubic regression spline with one knot at ξ can be obtained using a basis of the form $x, x^2, x^3, [x - \xi]_+^3$, where $[x - \xi]_+^3 = (x - \xi)^3$ if $x > \xi$ and equals 0 otherwise. We will now show that a function of the form

$$f(x) = \beta_0 + \beta_1 x + \beta_2 x^2 + \beta_3 x^3 + \beta_4 [x - \xi]_+^3$$

is indeed a cubic regression spline, regardless of the values of $\beta_0, \beta_1, \beta_2, \beta_3, \beta_4$.

1. Find a cubic polynomial

$$f_1(x) = a_1 + b_1 x + c_1 x^2 + d_1 x^3$$

such that $f(x) = f_1(x)$ for all $x \leq \xi$. Express a_1, b_1, c_1, d_1 in terms of $\beta_0, \beta_1, \beta_2, \beta_3, \beta_4$.

- Find a cubic polynomial

$$f_2(x) = a_2 + b_2x + c_2x^2 + d_2x^3$$

such that $f(x) = f_2(x)$ for all $x > \xi$. Express a_2, b_2, c_2, d_2 in terms of $\beta_0, \beta_1, \beta_2, \beta_3, \beta_4$. We have now established that $f(x)$ is a piece-wise polynomial.

- Show that $f_1(\xi) = f_2(\xi)$. That is, $f(x)$ is continuous at ξ .

Solution

- The values are:

$$a_1 = \beta_0, \quad b_1 = \beta_1, \quad c_1 = \beta_2, \quad d_1 = \beta_3$$

- Recall that:

$$(x - \xi)^3 = x^3 - \xi^3 + 3x\xi^2 - 3x^2\xi$$

Then, the values are:

$$a_2 = (\beta_0 - \beta_4\xi^3),$$

$$b_2 = (\beta_1 + 3\beta_4\xi^2),$$

$$c_2 = (\beta_2 - 3\beta_4\xi),$$

$$d_2 = \beta_3 + \beta_4$$

- Follows by algebraic manipulation, or simply from the fact that $[x - \xi]^3 = 0$ when $x = \xi$.

Problem 3

You will now derive the Bayesian connection to the ridge regression discussed in Section 6.2.2. of ISL.

- Suppose that $y_i = \beta_0 + \sum_{j=1}^p x_{ij}\beta_j + \epsilon_i$ where $\epsilon_1, \dots, \epsilon_n$ are independent and identically distributed from a normal distribution $N(0, 1)$. Write out the likelihood for the data as a function of values β .
- Assume the following prior for β : β_1, \dots, β_p are independent and identically distributed according to a normal distribution with mean zero and variance c . Write out the posterior for β in this setting using Bayes theorem.
- Argue that the ridge regression estimate is the value of β with maximal probability under this posterior distribution. Compute log of the probability in order to make this point. *Hint: The denominator (= the probability of data) can be ignored in computing the maximum probability.*

Solution

- The likelihood function is:

$$\frac{1}{(2\pi)^{n/2}} \prod_{i=1}^n e^{-\frac{\epsilon_i^2}{2}} = \frac{1}{(2\pi)^{n/2}} \prod_{i=1}^n e^{-\frac{(y_i - \beta_0 + \sum_{j=1}^p x_{ij}\beta_j)^2}{2}}$$

- To simplify the notation, I will use y to denote the random variable representing data. The posterior is:

$$P(\beta|y) = \frac{P(y|\beta)P(\beta)}{P(y)} = \frac{1}{P(y)} \frac{1}{(2\pi)^{n/2}} \prod_{i=1}^n e^{-\frac{(y_i - \beta_0 + \sum_{j=1}^p x_{ij}\beta_j)^2}{2}} \frac{1}{(2\pi c)^{n/2}} \prod_{j=1}^p e^{-\frac{\beta_j^2}{2c}}$$

- Take the log of the posterior probability to get:

$$-\frac{1}{2} \sum_{i=1}^n \left(y_i - \beta_0 + \sum_{j=1}^p x_{ij} \beta_j \right)^2 - \frac{1}{2c} \sum_{j=1}^p \beta_j^2 + O(1)$$

Here, $O(1)$ denotes all the terms that do not depend on β . So to maximize this expression, we need to solve the following minimization problem:

$$\min_{\beta} \sum_{i=1}^n \left(y_i - \beta_0 + \sum_{j=1}^p x_{ij} \beta_j \right)^2 + \frac{1}{c} \sum_{j=1}^p \beta_j^2 = \min_{\beta} \sum_{i=1}^n \text{RSS} + \frac{1}{c} \sum_{j=1}^p \beta_j^2 ,$$

which is the same as ridge regression.